p256: wip: use generic bignum lib for LowLevel

code/ecdsap256/Hacl.Impl.P256.LowLevel.fst
@@ -1,231 +1,148 @@
 module Hacl.Impl.P256.LowLevel
 
+open FStar.Mul
 open FStar.HyperStack.All
 open FStar.HyperStack
 module ST = FStar.HyperStack.ST
 
-open FStar.Mul
-open FStar.Math
-open FStar.Math.Lemmas
-
 open Lib.IntTypes
 open Lib.Buffer
 open Lib.ByteBuffer
-
-open Spec.P256.Definitions
-open Spec.P256.Lemmas
-open Spec.ECDSA
-open Hacl.Spec.P256.Felem
-
 open Lib.IntTypes.Intrinsics
 
-#set-options "--fuel 0 --ifuel 0 --z3rlimit 200"
+open Hacl.Spec.P256.Felem
+module BN = Hacl.Bignum
+module SN = Hacl.Spec.Bignum
 
-val isZero_uint64_CT:  f: felem -> Stack uint64
+#set-options "--z3rlimit 50 --fuel 0 --ifuel 0"
+
+inline_for_extraction noextract
+val mul: f:felem -> r:felem -> out:widefelem -> Stack unit
+  (requires fun h ->
+    live h out /\ live h f /\ live h r /\
+    eq_or_disjoint r f /\ disjoint f out /\ disjoint r out)
+  (ensures  fun h0 _ h1 -> modifies (loc out) h0 h1 /\
+    wide_as_nat h1 out = as_nat h0 r * as_nat h0 f)
+
+let mul f r out =
+  let h0 = ST.get () in
+  BN.bn_mul #U64 4ul 4ul f r out;
+  let h1 = ST.get () in
+  SN.bn_mul_lemma (as_seq h0 f) (as_seq h0 r);
+  bignum_bn_v_is_as_nat h0 f;
+  bignum_bn_v_is_as_nat h0 r;
+  bignum_bn_v_is_wide_as_nat h1 out
+
+
+val sq: f:felem -> out:widefelem -> Stack unit
+  (requires fun h ->
+    live h out /\ live h f /\ eq_or_disjoint f out)
+  (ensures  fun h0 _ h1 -> modifies (loc out) h0 h1 /\
+    wide_as_nat h1 out = as_nat h0 f * as_nat h0 f)
+
+let sq f out =
+  let h0 = ST.get () in
+  BN.bn_sqr #U64 4ul f out;
+  let h1 = ST.get () in
+  SN.bn_sqr_lemma (as_seq h0 f);
+  bignum_bn_v_is_as_nat h0 f;
+  bignum_bn_v_is_wide_as_nat h1 out
+
+
+val isZero_uint64_CT: f:felem -> Stack uint64
   (requires fun h -> live h f)
-  (ensures fun h0 r h1 -> modifies0 h0 h1 /\ (if as_nat h0 f = 0 then uint_v r == pow2 64 - 1 else uint_v r == 0))
+  (ensures fun h0 r h1 -> modifies0 h0 h1 /\
+    (if as_nat h0 f = 0 then uint_v r == pow2 64 - 1 else uint_v r == 0))
 
 let isZero_uint64_CT f =
-  let a0 = index f (size 0) in
-  let a1 = index f (size 1) in
-  let a2 = index f (size 2) in
-  let a3 = index f (size 3) in
-
-  let r0 = eq_mask a0 (u64 0) in
-  let r1 = eq_mask a1 (u64 0) in
-  let r2 = eq_mask a2 (u64 0) in
-  let r3 = eq_mask a3 (u64 0) in
-
-  let r01 = logand r0 r1 in
-     logand_lemma r0 r1;
-  let r23 = logand r2 r3 in
-     logand_lemma r2 r3;
-  let r = logand r01 r23 in
-    logand_lemma r01 r23;
-  r
+  let h0 = ST.get () in
+  SN.bn_is_zero_mask_lemma (as_seq h0 f);
+  bignum_bn_v_is_as_nat h0 f;
+  BN.bn_is_zero_mask #U64 4ul f
 
 
-val compare_felem: a: felem -> b: felem -> Stack uint64
+val compare_felem: a:felem -> b:felem -> Stack uint64
   (requires fun h -> live h a /\ live h b)
-  (ensures fun h0 r h1 -> modifies0 h0 h1 /\ (if as_nat h0 a = as_nat h0 b then uint_v r == pow2 64 - 1 else uint_v r = 0))
+  (ensures fun h0 r h1 -> modifies0 h0 h1 /\
+    (if as_nat h0 a = as_nat h0 b then uint_v r == pow2 64 - 1 else uint_v r = 0))
 
 let compare_felem a b =
-  let a_0 = index a (size 0) in
-  let a_1 = index a (size 1) in
-  let a_2 = index a (size 2) in
-  let a_3 = index a (size 3) in
-
-  let b_0 = index b (size 0) in
-  let b_1 = index b (size 1) in
-  let b_2 = index b (size 2) in
-  let b_3 = index b (size 3) in
-
-  let r_0 = eq_mask a_0 b_0 in
-      eq_mask_lemma a_0 b_0;
-  let r_1 = eq_mask a_1 b_1 in
-      eq_mask_lemma a_1 b_1;
-  let r_2 = eq_mask a_2 b_2 in
-      eq_mask_lemma a_2 b_2;
-  let r_3 = eq_mask a_3 b_3 in
-      eq_mask_lemma a_3 b_3;
-
-  let r01 = logand r_0 r_1 in
-      logand_lemma r_0 r_1;
-  let r23 = logand r_2 r_3 in
-      logand_lemma r_2 r_3;
-
-  let r = logand r01 r23 in
-      logand_lemma r01 r23;
-      lemma_equality (a_0, a_1, a_2, a_3) (b_0, b_1, b_2, b_3);
-  r
+  let h0 = ST.get () in
+  SN.bn_eq_mask_lemma (as_seq h0 a) (as_seq h0 b);
+  bignum_bn_v_is_as_nat h0 a;
+  bignum_bn_v_is_as_nat h0 b;
+  BN.bn_eq_mask #U64 4ul a b
 
 
-val copy_conditional: out: felem -> x: felem -> mask: uint64{uint_v mask = 0 \/ uint_v mask = pow2 64 - 1} -> Stack unit
-  (requires fun h -> live h out /\ live h x)
+// NOTE: changed precondition `eq_or_disjoint out x`
+val copy_conditional: out:felem -> x:felem
+  -> mask:uint64{uint_v mask = 0 \/ uint_v mask = pow2 64 - 1} -> Stack unit
+  (requires fun h -> live h out /\ live h x /\ eq_or_disjoint out x)
   (ensures fun h0 _ h1 -> modifies (loc out) h0 h1 /\
-    (if uint_v mask = 0 then as_seq h1 out == as_seq h0 out else as_seq h1 out == as_seq h0 x)
-  )
+    (if uint_v mask = 0 then as_seq h1 out == as_seq h0 out else as_seq h1 out == as_seq h0 x))
 
 let copy_conditional out x mask =
-    let h0 = ST.get() in
-  let out_0 = index out (size 0) in
-  let out_1 = index out (size 1) in
-  let out_2 = index out (size 2) in
-  let out_3 = index out (size 3) in
-
-  let x_0 = index x (size 0) in
-  let x_1 = index x (size 1) in
-  let x_2 = index x (size 2) in
-  let x_3 = index x (size 3) in
-
-  let r_0 = logxor out_0 (logand mask (logxor out_0 x_0)) in
-  let r_1 = logxor out_1 (logand mask (logxor out_1 x_1)) in
-  let r_2 = logxor out_2 (logand mask (logxor out_2 x_2)) in
-  let r_3 = logxor out_3 (logand mask (logxor out_3 x_3)) in
-
-  lemma_xor_copy_cond out_0 x_0 mask;
-  lemma_xor_copy_cond out_1 x_1 mask;
-  lemma_xor_copy_cond out_2 x_2 mask;
-  lemma_xor_copy_cond out_3 x_3 mask;
-
-  upd out (size 0) r_0;
-  upd out (size 1) r_1;
-  upd out (size 2) r_2;
-  upd out (size 3) r_3;
-    let h1 = ST.get() in
-
-  lemma_eq_funct_ (as_seq h1 out) (as_seq h0 out);
-  lemma_eq_funct_ (as_seq h1 out) (as_seq h0 x)
+  buf_mask_select x out mask out
 
 
-val add4: x: felem -> y: felem -> result: felem ->
+val cmovznz4: cin:uint64 -> x:felem -> y:felem -> out:felem -> Stack unit
+  (requires fun h ->
+    live h x /\ live h y /\ live h out /\
+    disjoint x out /\ eq_or_disjoint y out)
+  (ensures fun h0 _ h1 -> modifies1 out h0 h1 /\
+    (if uint_v cin = 0 then as_nat h1 out == as_nat h0 x else as_nat h1 out == as_nat h0 y))
+
+let cmovznz4 cin x y out =
+  let mask = neq_mask cin (u64 0) in
+  buf_mask_select y x mask out
+
+
+// NOTE: changed precondition `eq_or_disjoint x y`
+val add4: x:felem -> y:felem -> out:felem -> Stack uint64
+  (requires fun h ->
+    live h x /\ live h y /\ live h out /\
+    eq_or_disjoint x y /\ eq_or_disjoint x out /\ eq_or_disjoint y out)
+  (ensures fun h0 c h1 -> modifies (loc out) h0 h1 /\ v c <= 1 /\
+    as_nat h1 out + v c * pow2 256 == as_nat h0 x + as_nat h0 y)
+
+let add4 x y out =
+  let h0 = ST.get () in
+  let c = BN.bn_add_eq_len 4ul x y out in
+  let h1 = ST.get () in
+  SN.bn_add_lemma (as_seq h0 x) (as_seq h0 y);
+  bignum_bn_v_is_as_nat h0 x;
+  bignum_bn_v_is_as_nat h0 y;
+  bignum_bn_v_is_as_nat h1 out;
+  c
+
+
+// NOTE: changed precondition `eq_or_disjoint x y`
+val add8: x:widefelem -> y:widefelem -> out:widefelem -> Stack uint64
+  (requires fun h ->
+    live h x /\ live h y /\ live h out /\
+    eq_or_disjoint x y /\ eq_or_disjoint x out /\ eq_or_disjoint y out)
+  (ensures fun h0 c h1 -> modifies (loc out) h0 h1 /\ v c <= 1 /\
+    wide_as_nat h1 out + v c * pow2 512 == wide_as_nat h0 x + wide_as_nat h0 y)
+
+let add8 x y out =
+  let h0 = ST.get () in
+  let c = BN.bn_add_eq_len 8ul x y out in
+  let h1 = ST.get () in
+  SN.bn_add_lemma (as_seq h0 x) (as_seq h0 y);
+  bignum_bn_v_is_wide_as_nat h0 x;
+  bignum_bn_v_is_wide_as_nat h0 y;
+  bignum_bn_v_is_wide_as_nat h1 out;
+  c
+
+
+val add4_variables: x:felem -> cin:uint64{uint_v cin <= 1}
+  -> y0:uint64 -> y1:uint64 -> y2:uint64 -> y3:uint64 -> result:felem ->
   Stack uint64
-    (requires fun h -> live h x /\ live h y /\ live h result /\ eq_or_disjoint x result /\ eq_or_disjoint y result)
-    (ensures fun h0 c h1 -> modifies (loc result) h0 h1 /\ v c <= 1 /\
-      as_nat h1 result + v c * pow2 256 == as_nat h0 x + as_nat h0 y)
-
-let add4 x y result =
-  let h0 = ST.get() in
-
-  let r0 = sub result (size 0) (size 1) in
-  let r1 = sub result (size 1) (size 1) in
-  let r2 = sub result (size 2) (size 1) in
-  let r3 = sub result (size 3) (size 1) in
-
-    assert(let r1_0 = as_seq h0 r1 in let r0_ = as_seq h0 result in Seq.index r0_ 1 == Seq.index r1_0 0);
-    assert(let r2_0 = as_seq h0 r2 in let r0_ = as_seq h0 result in Seq.index r0_ 2 == Seq.index r2_0 0);
-    assert(let r3_0 = as_seq h0 r3 in let r0_ = as_seq h0 result in Seq.index r0_ 3 == Seq.index r3_0 0);
-
-
-  let cc0 = add_carry_u64 (u64 0) x.(0ul) y.(0ul) r0 in
-  let cc1 = add_carry_u64 cc0 x.(1ul) y.(1ul) r1 in
-  let cc2 = add_carry_u64 cc1 x.(2ul) y.(2ul) r2 in
-  let cc3 = add_carry_u64 cc2 x.(3ul) y.(3ul) r3 in
-
-  assert_norm (pow2 64 * pow2 64 = pow2 128);
-  assert_norm (pow2 64 * pow2 64 * pow2 64 = pow2 192);
-  assert_norm (pow2 64 * pow2 64 * pow2 64 * pow2 64 = pow2 256);
-
-  cc3
-
-// local function
-val add4_with_carry: c: uint64 ->  x: felem -> y: felem -> result: felem ->
-  Stack uint64
-    (requires fun h -> uint_v c <= 1 /\ live h x /\ live h y /\ live h result /\ eq_or_disjoint x result /\
-      eq_or_disjoint y result)
-    (ensures fun h0 carry h1 -> modifies (loc result) h0 h1 /\ uint_v carry <= 1 /\
-      as_nat h1 result + v carry * pow2 256 == as_nat h0 x + as_nat h0 y + uint_v c)
-
-let add4_with_carry c x y result =
-    let h0 = ST.get() in
-
-    let r0 = sub result (size 0) (size 1) in
-    let r1 = sub result (size 1) (size 1) in
-    let r2 = sub result (size 2) (size 1) in
-    let r3 = sub result (size 3) (size 1) in
-
-    let cc = add_carry_u64 c x.(0ul) y.(0ul) r0 in
-    let cc = add_carry_u64 cc x.(1ul) y.(1ul) r1 in
-    let cc = add_carry_u64 cc x.(2ul) y.(2ul) r2 in
-    let cc = add_carry_u64 cc x.(3ul) y.(3ul) r3 in
-
-      assert(let r1_0 = as_seq h0 r1 in let r0_ = as_seq h0 result in Seq.index r0_ 1 == Seq.index r1_0 0);
-      assert(let r2_0 = as_seq h0 r2 in let r0_ = as_seq h0 result in Seq.index r0_ 2 == Seq.index r2_0 0);
-      assert(let r3_0 = as_seq h0 r3 in let r0_ = as_seq h0 result in Seq.index r0_ 3 == Seq.index r3_0 0);
-
-      assert_norm (pow2 64 * pow2 64 = pow2 128);
-      assert_norm (pow2 64 * pow2 64 * pow2 64 = pow2 192);
-      assert_norm (pow2 64 * pow2 64 * pow2 64 * pow2 64 = pow2 256);
-
-    cc
-
-
-val add8: x: widefelem -> y: widefelem -> result: widefelem -> Stack uint64
-  (requires fun h -> live h x /\ live h y /\ live h result /\ eq_or_disjoint x result /\ eq_or_disjoint y result)
+  (requires fun h -> live h x /\ live h result /\ eq_or_disjoint x result)
   (ensures fun h0 c h1 -> modifies (loc result) h0 h1 /\ v c <= 1 /\
-    wide_as_nat h1 result + v c * pow2 512 == wide_as_nat h0 x + wide_as_nat h0 y)
-
-let add8 x y result =
-  assert_norm (pow2 64 * pow2 64 * pow2 64 * pow2 64 == pow2 256);
-
-  let h0 = ST.get() in
-    let a0 = sub x (size 0) (size 4) in
-    let a1 = sub x (size 4) (size 4) in
-
-    let b0 = sub y (size 0) (size 4) in
-    let b1 = sub y (size 4) (size 4) in
-
-    let c0 = sub result (size 0) (size 4) in
-    let c1 = sub result (size 4) (size 4) in
-
-    let carry0 = add4 a0 b0 c0 in
-    let carry1 = add4_with_carry carry0 a1 b1 c1 in
-      let h1 = ST.get() in
-
-    calc (==)
-    {
-      wide_as_nat h0 x + wide_as_nat h0 y;
-      (==)
-      {
-  distributivity_add_left (as_nat h0 a1) (as_nat h0 b1) (pow2 256)
-      }
-      wide_as_nat h1 result + uint_v carry1 * pow2 256 * pow2 256;
-      (==)
-      {
-  assert_norm (pow2 256 * pow2 256 = pow2 512)
-      }
-      wide_as_nat h1 result + uint_v carry1 * pow2 512;
-   };
-
-  carry1
-
-
-val add4_variables: x: felem -> cin: uint64 {uint_v cin <=1} ->  y0: uint64 -> y1: uint64 -> y2: uint64 -> y3: uint64 ->
-  result: felem ->
-  Stack uint64
-    (requires fun h -> live h x /\ live h result /\ eq_or_disjoint x result)
-    (ensures fun h0 c h1 -> modifies (loc result) h0 h1 /\ v c <= 1 /\
-      as_nat h1 result  + uint_v c * pow2 256 == as_nat h0 x + uint_v y0 + uint_v y1 * pow2 64 + uint_v y2 * pow2 128 + uint_v y3 * pow2 192 + uint_v cin)
+    as_nat h1 result  + uint_v c * pow2 256 ==
+    as_nat h0 x + uint_v y0 + uint_v y1 * pow2 64 +
+    uint_v y2 * pow2 128 + uint_v y3 * pow2 192 + uint_v cin)
 
 let add4_variables x cin y0 y1 y2 y3 result =
     let h0 = ST.get() in
@@ -251,15 +168,13 @@ let add4_variables x cin y0 y1 y2 y3 result =
     cc
 
 
-val sub4_il: x: felem -> y: glbuffer uint64 (size 4) -> result: felem ->
-  Stack uint64
-    (requires fun h -> live h x /\ live h y /\ live h result /\ disjoint x result /\ disjoint result y)
-    (ensures fun h0 c h1 -> modifies1 result h0 h1 /\ v c <= 1 /\
-      (
-  as_nat h1 result - v c * pow2 256 == as_nat h0 x  - as_nat_il h0 y /\
-  (if uint_v c = 0 then as_nat h0 x >= as_nat_il h0 y else as_nat h0 x < as_nat_il h0 y)
-      )
-    )
+val sub4_il: x:felem -> y:glbuffer uint64 (size 4) -> result:felem -> Stack uint64
+  (requires fun h ->
+    live h x /\ live h y /\ live h result /\
+    disjoint x result /\ disjoint result y)
+  (ensures fun h0 c h1 -> modifies1 result h0 h1 /\ v c <= 1 /\
+    as_nat h1 result - v c * pow2 256 == as_nat h0 x - as_nat_il h0 y /\
+    (if uint_v c = 0 then as_nat h0 x >= as_nat_il h0 y else as_nat h0 x < as_nat_il h0 y))
 
 let sub4_il x y result =
     let r0 = sub result (size 0) (size 1) in
@@ -279,37 +194,28 @@ let sub4_il x y result =
     cc
 
 
-val sub4: x: felem -> y:felem -> result: felem ->
-  Stack uint64
-    (requires fun h -> live h x /\ live h y /\ live h result /\ eq_or_disjoint x result /\ eq_or_disjoint y result)
-    (ensures fun h0 c h1 -> modifies1 result h0 h1 /\ v c <= 1 /\ as_nat h1 result - v c * pow2 256 == as_nat h0 x - as_nat h0 y)
+// NOTE: changed precondition `eq_or_disjoint x y`
+val sub4: x:felem -> y:felem -> out:felem -> Stack uint64
+  (requires fun h ->
+    live h x /\ live h y /\ live h out /\
+    eq_or_disjoint x y /\ eq_or_disjoint x out /\ eq_or_disjoint y out)
+  (ensures fun h0 c h1 -> modifies1 out h0 h1 /\ v c <= 1 /\
+    as_nat h1 out - v c * pow2 256 == as_nat h0 x - as_nat h0 y)
 
-let sub4 x y result =
-  let h0 = ST.get() in
-
-  let r0 = sub result (size 0) (size 1) in
-  let r1 = sub result (size 1) (size 1) in
-  let r2 = sub result (size 2) (size 1) in
-  let r3 = sub result (size 3) (size 1) in
-
-  let cc = sub_borrow_u64 (u64 0) x.(size 0) y.(size 0) r0 in
-  let cc = sub_borrow_u64 cc x.(size 1) y.(size 1) r1 in
-  let cc = sub_borrow_u64 cc x.(size 2) y.(size 2) r2 in
-  let cc = sub_borrow_u64 cc x.(size 3) y.(size 3) r3 in
-
-    assert(let r1_0 = as_seq h0 r1 in let r0_ = as_seq h0 result in Seq.index r0_ 1 == Seq.index r1_0 0);
-    assert(let r2_0 = as_seq h0 r2 in let r0_ = as_seq h0 result in Seq.index r0_ 2 == Seq.index r2_0 0);
-    assert(let r3_0 = as_seq h0 r3 in let r0_ = as_seq h0 result in Seq.index r0_ 3 == Seq.index r3_0 0);
-
-    assert_norm (pow2 64 * pow2 64 = pow2 128);
-    assert_norm (pow2 64 * pow2 64 * pow2 64 = pow2 192);
-    assert_norm (pow2 64 * pow2 64 * pow2 64 * pow2 64 = pow2 256);
-
-  cc
+let sub4 x y out =
+  let h0 = ST.get () in
+  let c = BN.bn_sub_eq_len 4ul x y out in
+  let h1 = ST.get () in
+  SN.bn_sub_lemma (as_seq h0 x) (as_seq h0 y);
+  bignum_bn_v_is_as_nat h0 x;
+  bignum_bn_v_is_as_nat h0 y;
+  bignum_bn_v_is_as_nat h1 out;
+  c
 
 
-val mul64: x: uint64 -> y: uint64 -> result: lbuffer uint64 (size 1) -> temp: lbuffer uint64 (size 1) ->
-  Stack unit
+// TODO: mv
+val mul64: x:uint64 -> y:uint64
+  -> result:lbuffer uint64 (size 1) -> temp:lbuffer uint64 (size 1) -> Stack unit
   (requires fun h -> live h result /\ live h temp /\ disjoint result temp)
   (ensures fun h0 _ h1 -> modifies (loc result |+| loc temp) h0 h1 /\ (
     let h0 = Seq.index (as_seq h1 temp) 0 in
@@ -324,18 +230,163 @@ let mul64 x y result temp =
 
 
 // local function
-inline_for_extraction noextract
-val mult64_0: x: felem -> u: uint64 -> result: lbuffer uint64 (size 1) -> temp: lbuffer uint64 (size 1) -> Stack unit
-  (requires fun h -> live h x /\ live h result /\ live h temp /\ disjoint result temp)
-  (ensures fun h0 _ h1 ->
-    let result_ = Seq.index (as_seq h1 result) 0 in
-    let c = Seq.index (as_seq h1 temp) 0 in
-    let f0 = Seq.index (as_seq h0 x) 0 in
-    uint_v result_ + uint_v c * pow2 64 = uint_v f0 * uint_v u /\ modifies (loc result |+| loc temp) h0 h1)
+val lemma_shift_256: a: int -> b: int -> c: int -> d: int -> Lemma (
+    a * pow2 64 * pow2 64 * pow2 64 * pow2 64 +
+    b * pow2 64 * pow2 64 * pow2 64 * pow2 64 * pow2 64 +
+    c * pow2 64 * pow2 64 * pow2 64 * pow2 64 * pow2 64 * pow2 64  +
+    d * pow2 64 * pow2 64 * pow2 64 * pow2 64 * pow2 64 * pow2 64 * pow2 64 ==
+    (a + b * pow2 64 + c * pow2 64 * pow2 64 + d * pow2 64 * pow2 64 * pow2 64) * pow2 64 * pow2 64 * pow2 64 * pow2 64)
 
-let mult64_0 x u result temp =
-  let f0 = index x (size 0) in
-  mul64 f0 u result temp
+let lemma_shift_256 a b c d = ()
+
+
+// TODO: add bn_lshift
+val shift_256_impl: i:felem -> o:lbuffer uint64 (size 8) -> Stack unit
+  (requires fun h ->
+    live h i /\ live h o /\ disjoint i o)
+  (ensures fun h0 _ h1 -> modifies1 o h0 h1 /\
+    wide_as_nat h1 o == as_nat h0 i * pow2 256)
+
+let shift_256_impl i o =
+  assert_norm (pow2 64 * pow2 64 * pow2 64 * pow2 64 = pow2 256);
+
+  let h0 = ST.get() in
+    upd o (size 0) (u64 0);
+    upd o (size 1) (u64 0);
+    upd o (size 2) (u64 0);
+    upd o (size 3) (u64 0);
+    upd o (size 4) i.(size 0);
+    upd o (size 5) i.(size 1);
+    upd o (size 6) i.(size 2);
+    upd o (size 7) i.(size 3);
+
+  lemma_shift_256
+    (v (Lib.Sequence.index (as_seq h0 i) 0))
+    (v (Lib.Sequence.index (as_seq h0 i) 1))
+    (v (Lib.Sequence.index (as_seq h0 i) 2))
+    (v (Lib.Sequence.index (as_seq h0 i) 3))
+
+
+inline_for_extraction noextract
+val mod64: a:widefelem -> Stack uint64
+  (requires fun h -> live h a)
+  (ensures fun h0 r h1 -> modifies0 h0 h1 /\
+    wide_as_nat h1 a % pow2 64 = uint_v r)
+
+let mod64 a =
+  let h0 = ST.get () in
+  let r = index a (size 0) in
+  bignum_bn_v_is_wide_as_nat h0 a;
+  Hacl.Spec.Bignum.Definitions.bn_eval_index (as_seq h0 a) 0;
+  assert (v r == wide_as_nat h0 a / pow2 0 % pow2 64);
+  r
+
+
+val shift8: t:widefelem -> out:widefelem -> Stack unit
+  (requires fun h ->
+    live h t /\ live h out /\ eq_or_disjoint t out)
+  (ensures fun h0 _ h1 -> modifies (loc out) h0 h1 /\
+    wide_as_nat h0 t / pow2 64 = wide_as_nat h1 out)
+
+let shift8 t out =
+  let t1 = index t (size 1) in
+  let t2 = index t (size 2) in
+  let t3 = index t (size 3) in
+  let t4 = index t (size 4) in
+  let t5 = index t (size 5) in
+  let t6 = index t (size 6) in
+  let t7 = index t (size 7) in
+
+  upd out (size 0) t1;
+  upd out (size 1) t2;
+  upd out (size 2) t3;
+  upd out (size 3) t4;
+  upd out (size 4) t5;
+  upd out (size 5) t6;
+  upd out (size 6) t7;
+  upd out (size 7) (u64 0)
+
+
+// TODO: mv
+inline_for_extraction noextract
+val scalar_bit:
+    #buf_type: buftype ->
+    s:lbuffer_t buf_type uint8 (size 32)
+  -> n:size_t{v n < 256}
+  -> Stack uint64
+    (requires fun h0 -> live h0 s)
+    (ensures  fun h0 r h1 -> h0 == h1 /\
+      r == Spec.ECDSA.ith_bit (as_seq h0 s) (v n) /\ v r <= 1)
+
+let scalar_bit #buf_type s n =
+  let h0 = ST.get () in
+  mod_mask_lemma ((Lib.Sequence.index (as_seq h0 s) (v n / 8)) >>. (n %. 8ul)) 1ul;
+  assert_norm (1 = pow2 1 - 1);
+  assert (v (mod_mask #U8 #SEC 1ul) == v (u8 1));
+  to_u64 ((s.(n /. 8ul) >>. (n %. 8ul)) &. u8 1)
+
+
+val uploadZeroImpl: f:felem -> Stack unit
+  (requires fun h -> live h f)
+  (ensures fun h0 _ h1 -> modifies (loc f) h0 h1 /\
+    as_nat h1 f == 0)
+
+let uploadZeroImpl f =
+  upd f (size 0) (u64 0);
+  upd f (size 1) (u64 0);
+  upd f (size 2) (u64 0);
+  upd f (size 3) (u64 0)
+
+
+val uploadOneImpl: f:felem -> Stack unit
+  (requires fun h -> live h f)
+  (ensures fun h0 _ h1 -> modifies (loc f) h0 h1 /\
+    as_nat h1 f == 1)
+
+let uploadOneImpl f =
+  upd f (size 0) (u64 1);
+  upd f (size 1) (u64 0);
+  upd f (size 2) (u64 0);
+  upd f (size 3) (u64 0)
+
+
+val toUint8: i:felem -> o:lbuffer uint8 (32ul) -> Stack unit
+  (requires fun h -> live h i /\ live h o /\ disjoint i o)
+  (ensures fun h0 _ h1 -> modifies (loc o) h0 h1 /\
+    as_seq h1 o == Lib.ByteSequence.uints_to_bytes_be #_ #_ #4 (as_seq h0 i))
+
+let toUint8 i o =
+  Lib.ByteBuffer.uints_to_bytes_be (size 4) o i
+
+
+val changeEndian: i:felem -> Stack unit
+  (requires fun h -> live h i)
+  (ensures  fun h0 _ h1 -> modifies1 i h0 h1 /\
+    as_seq h1 i == Spec.ECDSA.changeEndian (as_seq h0 i) /\
+    as_nat h1 i < pow2 256)
+
+let changeEndian i =
+  assert_norm (pow2 64 * pow2 64 = pow2 (2 * 64));
+  assert_norm (pow2 (2 * 64) * pow2 64 = pow2 (3 * 64));
+  assert_norm (pow2 (3 * 64) * pow2 64 = pow2 (4 * 64));
+  let zero = index i (size 0) in
+  let one = index i (size 1) in
+  let two = index i (size 2) in
+  let three = index i (size 3) in
+  upd i (size 0) three;
+  upd i (size 1) two;
+  upd i (size 2) one;
+  upd i (size 3) zero
+
+
+val toUint64ChangeEndian: i:lbuffer uint8 (size 32) -> o:felem -> Stack unit
+  (requires fun h -> live h i /\ live h o /\ disjoint i o)
+  (ensures  fun h0 _ h1 -> modifies (loc o) h0 h1 /\
+    as_seq h1 o == Spec.ECDSA.changeEndian (Lib.ByteSequence.uints_from_bytes_be (as_seq h0 i)))
+
+let toUint64ChangeEndian i o =
+  Lib.ByteBuffer.uints_from_bytes_be o i;
+  changeEndian o
 
 
 // local function
@@ -410,9 +461,9 @@ let mul1_il f u result =
   let c3 = mult64_c f3 u c2 o3 temp in
     let h4 = ST.get() in
   let temp0 = index temp (size 0) in
-    lemma_low_level0 (uint_v(Seq.index (as_seq h1 o0) 0)) (uint_v (Seq.index (as_seq h2 o1) 0)) (uint_v (Seq.index (as_seq h3 o2) 0)) (uint_v (Seq.index (as_seq h4 o3) 0)) (uint_v f0) (uint_v f1) (uint_v f2) (uint_v f3) (uint_v u) (uint_v (Seq.index (as_seq h2 temp) 0)) (uint_v c1) (uint_v c2) (uint_v c3) (uint_v (Seq.index (as_seq h3 temp) 0)) (uint_v temp0);
+    Spec.P256.Lemmas.lemma_low_level0 (uint_v(Seq.index (as_seq h1 o0) 0)) (uint_v (Seq.index (as_seq h2 o1) 0)) (uint_v (Seq.index (as_seq h3 o2) 0)) (uint_v (Seq.index (as_seq h4 o3) 0)) (uint_v f0) (uint_v f1) (uint_v f2) (uint_v f3) (uint_v u) (uint_v (Seq.index (as_seq h2 temp) 0)) (uint_v c1) (uint_v c2) (uint_v c3) (uint_v (Seq.index (as_seq h3 temp) 0)) (uint_v temp0);
 
-  mul_lemma_4 (as_nat_il h0 f) (uint_v u) (pow2 256 - 1) (pow2 64 - 1);
+  Spec.P256.Lemmas.mul_lemma_4 (as_nat_il h0 f) (uint_v u) (pow2 256 - 1) (pow2 64 - 1);
   assert_norm((pow2 256 - 1) * (pow2 64 - 1) == pow2 320 - pow2 256 - pow2 64 + 1);
   assert_norm((pow2 320 - pow2 256) / pow2 256 == pow2 64 - 1);
 
@@ -421,133 +472,9 @@ let mul1_il f u result =
 
 
 inline_for_extraction noextract
-val mul: f: felem -> r: felem -> out: widefelem ->
-  Stack unit
-  (requires fun h -> live h out /\ live h f /\ live h r /\ eq_or_disjoint r f /\ disjoint f out /\ disjoint r out)
-  (ensures  fun h0 _ h1 -> modifies (loc out) h0 h1 /\
-    wide_as_nat h1 out = as_nat h0 r * as_nat h0 f)
-
-let mul f r out =
-  let h0 = ST.get() in
-    Hacl.Bignum.bn_mul #U64 4ul 4ul f r out;
-  let h1 = ST.get() in
-  Hacl.Spec.Bignum.bn_mul_lemma (as_seq h0 f) (as_seq h0 r);
-  bignum_bn_v_is_as_nat h0 f;
-  bignum_bn_v_is_as_nat h0 r;
-  bignum_bn_v_is_wide_as_nat h1 out
-
-
-// local function
-let lemma_mult_le_both (a b:nat) (n1 n2:nat):
-  Lemma (requires (a <= n1 /\ b <= n2))
-        (ensures (a * b <= n1 * n2)) = ()
-
-
-val sq: f: felem -> out: widefelem -> Stack unit
-    (requires fun h -> live h out /\ live h f /\ eq_or_disjoint f out)
-    (ensures  fun h0 _ h1 -> modifies (loc out) h0 h1 /\ wide_as_nat h1 out = as_nat h0 f * as_nat h0 f)
-
-let sq f out =
-  let h0 = ST.get() in
-    Hacl.Bignum.bn_sqr #U64 4ul f out;
-  let h1 = ST.get() in
-  Hacl.Spec.Bignum.bn_sqr_lemma (as_seq h0 f);
-  bignum_bn_v_is_as_nat h0 f;
-  bignum_bn_v_is_wide_as_nat h1 out
-
-
-val cmovznz4: cin: uint64 -> x: felem -> y: felem -> result: felem ->
-  Stack unit
-    (requires fun h -> live h x /\ live h y /\ live h result /\ disjoint x result /\ eq_or_disjoint y result)
-    (ensures fun h0 _ h1 -> modifies1 result h0 h1 /\
-      (if uint_v cin = 0 then as_nat h1 result == as_nat h0 x else as_nat h1 result == as_nat h0 y))
-
-let cmovznz4 cin x y r =
-  let h0 = ST.get() in
-  let mask = neq_mask cin (u64 0) in
-  let r0 = logor (logand y.(size 0) mask) (logand x.(size 0) (lognot mask)) in
-  let r1 = logor (logand y.(size 1) mask) (logand x.(size 1) (lognot mask)) in
-  let r2 = logor (logand y.(size 2) mask) (logand x.(size 2) (lognot mask)) in
-  let r3 = logor (logand y.(size 3) mask) (logand x.(size 3) (lognot mask)) in
-
-  upd r (size 0) r0;
-  upd r (size 1) r1;
-  upd r (size 2) r2;
-  upd r (size 3) r3;
-
-    let x = as_seq h0 x in
-    let y = as_seq h0 y in
-
-    cmovznz4_lemma cin (Seq.index x 0) (Seq.index y 0);
-    cmovznz4_lemma cin (Seq.index x 1) (Seq.index y 1);
-    cmovznz4_lemma cin (Seq.index x 2) (Seq.index y 2);
-    cmovznz4_lemma cin (Seq.index x 3) (Seq.index y 3)
-
-// local function
-val lemma_shift_256: a: int -> b: int -> c: int -> d: int -> Lemma (
-    a * pow2 64 * pow2 64 * pow2 64 * pow2 64 +
-    b * pow2 64 * pow2 64 * pow2 64 * pow2 64 * pow2 64 +
-    c * pow2 64 * pow2 64 * pow2 64 * pow2 64 * pow2 64 * pow2 64  +
-    d * pow2 64 * pow2 64 * pow2 64 * pow2 64 * pow2 64 * pow2 64 * pow2 64 ==
-    (a + b * pow2 64 + c * pow2 64 * pow2 64 + d * pow2 64 * pow2 64 * pow2 64) * pow2 64 * pow2 64 * pow2 64 * pow2 64)
-
-let lemma_shift_256 a b c d = ()
-
-
-val shift_256_impl: i: felem -> o: lbuffer uint64 (size 8) ->
-  Stack unit
-    (requires fun h -> live h i /\ live h o /\ disjoint i o)
-    (ensures fun h0 _ h1 -> modifies1 o h0 h1 /\ wide_as_nat h1 o == as_nat h0 i * pow2 256)
-
-let shift_256_impl i o =
-  assert_norm(pow2 64 * pow2 64 * pow2 64 * pow2 64 = pow2 256);
-
-  let h0 = ST.get() in
-    upd o (size 0) (u64 0);
-    upd o (size 1) (u64 0);
-    upd o (size 2) (u64 0);
-    upd o (size 3) (u64 0);
-    upd o (size 4) i.(size 0);
-    upd o (size 5) i.(size 1);
-    upd o (size 6) i.(size 2);
-    upd o (size 7) i.(size 3);
-
-  lemma_shift_256 (v (Lib.Sequence.index (as_seq h0 i) 0)) (v (Lib.Sequence.index (as_seq h0 i) 1)) (v (Lib.Sequence.index (as_seq h0 i) 2)) (v (Lib.Sequence.index (as_seq h0 i) 3))
-
-
-inline_for_extraction noextract
-val mod64: a: widefelem -> Stack uint64
-  (requires fun h -> live h a)
-  (ensures fun h0 r h1 -> modifies0 h0 h1 /\ wide_as_nat h1 a % pow2 64 = uint_v r)
-
-let mod64 a =
-  let r = index a (size 0) in
-    let h1 = ST.get() in
-  assert(
-   let open Lib.Sequence in
-   let s = as_seq h1 a in
-   let s0 = s.[0] in
-   let s1 = s.[1] in
-   let s2 = s.[2] in
-   let s3 = s.[3] in
-   let s4 = s.[4] in
-   let s5 = s.[5] in
-   let s6 = s.[6] in
-   let s7 = s.[7] in
-   wide_as_nat h1 a ==
-   v s0 + v s1 * pow2 64 + v s2 * pow2 64 * pow2 64 +
-   v s3 * pow2 64 * pow2 64 * pow2 64 +
-   v s4 * pow2 64 * pow2 64 * pow2 64 * pow2 64 +
-   v s5 * pow2 64 * pow2 64 * pow2 64 * pow2 64 * pow2 64 +
-   v s6 * pow2 64 * pow2 64 * pow2 64 * pow2 64 * pow2 64 * pow2 64 +
-   v s7 * pow2 64 * pow2 64 * pow2 64 * pow2 64 * pow2 64 * pow2 64 * pow2 64 /\
-   wide_as_nat h1 a % pow2 64 == v s0);
-  r
-
-
-inline_for_extraction noextract
-val shortened_mul: a: glbuffer uint64 (size 4) -> b: uint64 -> result: widefelem -> Stack unit
-  (requires fun h -> live h a /\ live h result /\ wide_as_nat h result = 0)
+val shortened_mul: a:glbuffer uint64 (size 4) -> b:uint64 -> result:widefelem -> Stack unit
+  (requires fun h ->
+    live h a /\ live h result /\ wide_as_nat h result = 0)
   (ensures fun h0 _ h1 -> modifies (loc result) h0 h1 /\
     as_nat_il h0 a * uint_v b = wide_as_nat h1 result /\
     wide_as_nat h1 result < pow2 320)
@@ -564,107 +491,3 @@ let shortened_mul a b result =
     assert(Lib.Sequence.index (as_seq h0 result) 7 == Lib.Sequence.index (as_seq h0 result48) 3);
 
     assert_norm( pow2 64 * pow2 64 * pow2 64 * pow2 64 = pow2 256)
-
-
-val shift8: t: widefelem -> t1: widefelem -> Stack unit
-  (requires fun h -> live h t /\ live h t1 /\ eq_or_disjoint t t1)
-  (ensures fun h0 _ h1 -> modifies (loc t1) h0 h1 /\ wide_as_nat h0 t / pow2 64 = wide_as_nat h1 t1)
-
-let shift8 t out =
-  let t1 = index t (size 1) in
-  let t2 = index t (size 2) in
-  let t3 = index t (size 3) in
-  let t4 = index t (size 4) in
-  let t5 = index t (size 5) in
-  let t6 = index t (size 6) in
-  let t7 = index t (size 7) in
-
-  upd out (size 0) t1;
-  upd out (size 1) t2;
-  upd out (size 2) t3;
-  upd out (size 3) t4;
-  upd out (size 4) t5;
-  upd out (size 5) t6;
-  upd out (size 6) t7;
-  upd out (size 7) (u64 0)
-
-(* this piece of code is taken from Hacl.Curve25519 *)
-inline_for_extraction noextract
-val scalar_bit:
-    #buf_type: buftype ->
-    s:lbuffer_t buf_type uint8 (size 32)
-  -> n:size_t{v n < 256}
-  -> Stack uint64
-    (requires fun h0 -> live h0 s)
-    (ensures  fun h0 r h1 -> h0 == h1 /\
-      r == ith_bit (as_seq h0 s) (v n) /\ v r <= 1)
-
-let scalar_bit #buf_type s n =
-  let h0 = ST.get () in
-  mod_mask_lemma ((Lib.Sequence.index (as_seq h0 s) (v n / 8)) >>. (n %. 8ul)) 1ul;
-  assert_norm (1 = pow2 1 - 1);
-  assert (v (mod_mask #U8 #SEC 1ul) == v (u8 1));
-  to_u64 ((s.(n /. 8ul) >>. (n %. 8ul)) &. u8 1)
-
-
-val uploadZeroImpl: f: felem -> Stack unit
-  (requires fun h -> live h f)
-  (ensures fun h0 _ h1 -> as_nat h1 f == 0 /\ modifies (loc f) h0 h1)
-
-let uploadZeroImpl f =
-  upd f (size 0) (u64 0);
-  upd f (size 1) (u64 0);
-  upd f (size 2) (u64 0);
-  upd f (size 3) (u64 0)
-
-val uploadOneImpl: f: felem -> Stack unit
-  (requires fun h -> live h f)
-  (ensures fun h0 _ h1 -> as_nat h1 f == 1 /\ modifies (loc f) h0 h1)
-
-let uploadOneImpl f =
-  upd f (size 0) (u64 1);
-  upd f (size 1) (u64 0);
-  upd f (size 2) (u64 0);
-  upd f (size 3) (u64 0)
-
-val toUint8: i: felem ->  o: lbuffer uint8 (32ul) -> Stack unit
-  (requires fun h -> live h i /\ live h o /\ disjoint i o)
-  (ensures fun h0 _ h1 ->
-    modifies (loc o) h0 h1 /\
-    as_seq h1 o == Lib.ByteSequence.uints_to_bytes_be #_ #_ #4 (as_seq h0 i)
-  )
-
-let toUint8 i o =
-  Lib.ByteBuffer.uints_to_bytes_be (size 4) o i
-
-
-val changeEndian: i:felem -> Stack unit
-  (requires fun h -> live h i)
-  (ensures  fun h0 _ h1 -> modifies1 i h0 h1 /\
-    as_seq h1 i == Spec.ECDSA.changeEndian (as_seq h0 i) /\
-    as_nat h1 i < pow2 256
-  )
-
-let changeEndian i =
-  assert_norm (pow2 64 * pow2 64 = pow2 (2 * 64));
-  assert_norm (pow2 (2 * 64) * pow2 64 = pow2 (3 * 64));
-  assert_norm (pow2 (3 * 64) * pow2 64 = pow2 (4 * 64));
-  let zero = index i (size 0) in
-  let one = index i (size 1) in
-  let two = index i (size 2) in
-  let three = index i (size 3) in
-  upd i (size 0) three;
-  upd i (size 1) two;
-  upd i (size 2) one;
-  upd i (size 3) zero
-
-val toUint64ChangeEndian: i:lbuffer uint8 (size 32) -> o:felem -> Stack unit
-  (requires fun h -> live h i /\ live h o /\ disjoint i o)
-  (ensures  fun h0 _ h1 ->
-    modifies (loc o) h0 h1 /\
-    as_seq h1 o == Spec.ECDSA.changeEndian (Lib.ByteSequence.uints_from_bytes_be (as_seq h0 i))
-  )
-
-let toUint64ChangeEndian i o =
-  Lib.ByteBuffer.uints_from_bytes_be o i;
-  changeEndian o
